tsyn fair merge

src/demo/fairmerge/Datatypes.thy
@@ -1,6 +1,6 @@
 theory Datatypes
 
-imports HOLCF
+imports inc.Prelude
 
 begin
 
@@ -13,25 +13,28 @@ datatype channel = cin1 | cin2 | cout | cbot
 section \<open>Message Definition\<close>
 
 text\<open>The same is true for the "Message" Datatype. Every kind of message has to be described here:\<close>
-datatype M = \<N> nat | \<B> bool | eps
+datatype M_pure = \<N> nat | \<B> bool
 
-text \<open>* Introduce symbol @{text ~} for empty time-slots called eps. \<close>
-syntax "@eps" :: M ("~")
-translations "~" == "CONST eps"
 
-instance M::countable
+instance M_pure::countable
   apply(countable_datatype)
   done
 
 text \<open>Then one describes the types of each channel. Only Messages included are allowed to be
   transmitted\<close>
-fun ctype :: "channel \<Rightarrow> M set" where 
-"ctype cin1 = range \<N>" |
-"ctype cin2 = range \<N>" |
-"ctype cout = range \<N>" |
-"ctype _ = {}"
+fun cMsg :: "channel \<Rightarrow> M_pure set" where 
+"cMsg cin1 = range \<N>" |
+"cMsg cin2 = range \<N>" |
+"cMsg cout = range \<N>" |
+"cMsg _ = {}"
 
-lemma ctypeempty_ex:"\<exists>c. ctype c = {}"
-  using ctype.simps by blast
+lemma cmsgempty_ex:"\<exists>c. cMsg c = {}"
+  using cMsg.simps by blast
+
+fun cTime :: "channel \<Rightarrow> timeType" where 
+"cTime cin1 = TTsyn" |
+"cTime cin2 = TTsyn" |
+"cTime cout = TTsyn" |
+"cTime _ = undefined"
 
 end
