src/demo/fairmerge/FMAutomat.thy
@@ -6,17 +6,39 @@ begin
 
 setup_lifting type_definition_ndAutomaton
 
-fun dAfm_case::"bool \<Rightarrow> nat list \<Rightarrow> nat list \<Rightarrow> (nat\<times> nat) \<Rightarrow> nat \<Rightarrow>(S_fm \<times> nat)"where
-"dAfm_case True  [] l2 (nat1,nat2) = (\<lambda>n. (S True  n []          (l2@[nat2]), nat1))"|
-"dAfm_case False l1 [] (nat1,nat2) = (\<lambda>n. (S False n (l1@[nat1]) []         , nat2))"|
+fun dAfm_case::"bool \<Rightarrow> nat list \<Rightarrow> nat list \<Rightarrow> (nat\<times> nat) \<Rightarrow> nat \<Rightarrow>(S_fm \<times> nat option)"where
+"dAfm_case True  [] l2 (nat1, nat2) = (\<lambda>n. (S True  n []          (l2@[nat2]),Some nat1))"|
+"dAfm_case False l1 [] (nat1, nat2) = (\<lambda>n. (S False n (l1@[nat1]) []         ,Some nat2))"|
 
-"dAfm_case True  (nhd#l1) l2       (nat1,nat2) = (\<lambda>n. (S True  n (l1@[nat1]) (l2@[nat2]),nhd))"|
-"dAfm_case False l1       (nhd#l2) (nat1,nat2) = (\<lambda>n. (S False n (l1@[nat1]) (l2@[nat2]),nhd))"
+"dAfm_case True  (nhd#l1) l2       (nat1, nat2) = (\<lambda>n. (S True  n (l1@[nat1]) (l2@[nat2]),Some nhd))"|
+"dAfm_case False l1       (nhd#l2) (nat1, nat2) = (\<lambda>n. (S False n (l1@[nat1]) (l2@[nat2]),Some nhd))"
+
+
+fun dAfm_case_option::"bool \<Rightarrow> nat list \<Rightarrow> nat list \<Rightarrow> (nat option\<times> nat option) \<Rightarrow> nat \<Rightarrow>(S_fm \<times> nat option)" where
+"dAfm_case_option bool l1 l2 (Some nat1, Some nat2) = dAfm_case bool l1 l2 (nat1, nat2)"|
+
+"dAfm_case_option bool [] [] (None            , None)      = (\<lambda>n. (S bool  n [] []        ,None     ))"|
+"dAfm_case_option bool [] [] (Some nat1       , None)      = (\<lambda>n. (S True  n [] []        ,Some nat1))"|
+"dAfm_case_option bool [] [] (None            , Some nat2) = (\<lambda>n. (S False n [] []        ,Some nat2))"|
+
+"dAfm_case_option False (nhd#l1) [] (None     , None)      = (\<lambda>n. (S True  n l1          []          ,Some nhd ))"|
+"dAfm_case_option True  (nhd#l1) l2 (None     , None)      = (\<lambda>n. (S True  n l1          l2          ,Some nhd ))"|
+"dAfm_case_option False (nhd#l1) [] (Some nat1, None)      = (\<lambda>n. (S True  n (l1@[nat1]) []          ,Some nhd ))"|
+"dAfm_case_option True  (nhd#l1) l2 (Some nat1, None)      = (\<lambda>n. (S True  n (l1@[nat1]) l2          ,Some nhd ))"|
+"dAfm_case_option True  (nhd#l1) l2 (None     , Some nat2) = (\<lambda>n. (S True  n l1          (l2@[nat2]) ,Some nhd ))"|
+"dAfm_case_option False l1       [] (None     , Some nat2) = (\<lambda>n. (S False n l1          []          ,Some nat2))"|
+
+"dAfm_case_option True  [] (nhd#l2) (None     , None)      = (\<lambda>n. (S False n []          l2          ,Some nhd ))"|
+"dAfm_case_option False l1 (nhd#l2) (None     , None)      = (\<lambda>n. (S False n l1          l2          ,Some nhd ))"|
+"dAfm_case_option False l1 (nhd#l2) (Some nat1, None)      = (\<lambda>n. (S False n (l1@[nat1]) l2          ,Some nhd ))"|
+"dAfm_case_option True  []  l2      (Some nat1, None)      = (\<lambda>n. (S True  n []          l2          ,Some nat1))"|
+"dAfm_case_option True  [] (nhd#l2) (None     , Some nat2) = (\<lambda>n. (S False n []          (l2@[nat2]) ,Some nhd ))"|
+"dAfm_case_option False l1 (nhd#l2) (None     , Some nat2) = (\<lambda>n. (S True  n l1          (l2@[nat2]) ,Some nhd ))"
 
 (*FM automaton*)
-fun dAfm_transition::"S_fm \<Rightarrow> (nat\<times> nat) \<Rightarrow> (S_fm \<times> nat)set"where
-"dAfm_transition (S bool 0       buf1 buf2) input = {(dAfm_case (\<not>bool) buf1 buf2 input) n | n. True} "|
-"dAfm_transition (S bool (Suc n) buf1 buf2) input = {(dAfm_case bool    buf1 buf2 input) n}"
+fun dAfm_transition::"S_fm \<Rightarrow> (nat option\<times> nat option) \<Rightarrow> (S_fm \<times> nat option )set"where
+"dAfm_transition (S bool 0       buf1 buf2) input = {(dAfm_case_option (\<not>bool) buf1 buf2 input) n | n. True} "|
+"dAfm_transition (S bool (Suc n) buf1 buf2) input = {(dAfm_case_option bool    buf1 buf2 input) n}"
 
 definition fairmergetransition::"(S_fm \<Rightarrow> inFM\<^sup>\<surd> \<Rightarrow> ((S_fm \<times> outFM\<^sup>\<Omega>) set))"where
 "fairmergetransition state insbe = ( let Set = (dAfm_transition state (fmInSBE.getter(insbe))) in
